First serious version is now working.
The next step is to move svm into a module and then have some examples in the
main.

src/svm.dfy
@@ -1,51 +1,41 @@
-include "util.dfy"
+include "util/int.dfy"	
+include "util/stack.dfy"
+include "util/memory.dfy"
+include "util/code.dfy"	
+
+import opened Int
 
 /**
  * Simple Virtual Machine consists of a stack, some random access 
  * memory, a sequence of bytecode instructions (and operands) and,
  * finally, a program counter.
  */
-type SVM = (stack<u16>,memory<u16>,seq<u8>,u16)
+datatype RawSVM = SVM(
+	stack:Stack.T<u16>,
+	mem:Memory.T<u16>,
+	code:Code.T<u8>,
+	pc:u16)
 
-/**
- * Extract stack from machine state.
- */ 
-function stck(vm:SVM) : stack<u16> { vm.0 }		
-
-/**
- * Extract data store from machine state.
- */
-function mem(vm:SVM) : memory<u16> { vm.1 }
-
-/**
- * Extract code sequence from machine state.
- */
-function code(vm:SVM) : seq<u8> { vm.2 }
-		
-/**
- * Extract program counter from machine state.
- */
-function pc(vm:SVM) : u16 { vm.3 }
-
-/**
- * Machine is considered to be halted if the program counter 
- * is out-of-bounds.
- */
-function halted(vm:SVM) : bool { pc(vm) >= (|code(vm)| as u16) }
-
-/**
- * Force the machine into a halted state.
- */
-function halt(vm:SVM) : SVM {
-		(vm.0,vm.1,vm.2,|vm.2| as u16)
-}
 /**
  * A valid Simple Virtual Machine requires a valid stack and a 
  * valid memory.  The program counter must also be valid with 
  * respect to the bytecode sequence.
  */		
-function validSVM(vm : SVM) : bool {
-		validStack(stck(vm)) && validMemory(mem(vm)) && pc(vm) <= |code(vm)|
+type SVM = vm:RawSVM | vm.pc <= Code.size(vm.code)
+witness SVM(stack:=Stack.empty(),mem:=Memory.empty(),code:=Code.empty(),pc:=0)
+	
+/**
+ * Machine is considered to be halted if the program counter 
+ * is out-of-bounds.
+ */
+function halted(vm:SVM) : bool { vm.pc >= Code.size(vm.code) }
+
+/**
+ * Force the machine into a halted state.
+ */
+function halt(vm:SVM) : SVM {
+	// Set pc to maximum position.
+	SVM(stack:=vm.stack, mem:=vm.mem, code:=vm.code, pc:=Code.size(vm.code))
 }
 
 // =============================================================================
@@ -70,54 +60,190 @@ const ADD:u8 := 0x05
 
 // Execute a "single step" of the current program.
 function step(vm:SVM) : SVM
-// Virtual machine must be valid		
-requires validSVM(vm)
-// Virtual machine cannot be halted.
-requires !halted(vm) {
-				// decode
-				var opcode : u8 := svm_decode(vm);
-				//
-				var vm':SVM := svm_goto(vm, pc(vm)+1);
-				//
-				if opcode == NOP
-				then
-						stepNOP(vm')
-				else
-						// Opcodes requiring operand
-						var k : u8 := svm_decode(vm');
-						var vm'':SVM := svm_goto(vm', pc(vm')+1);
-						//
-						stepLDC(vm'',k)
-				// else
-				// 		halt(vm')
+	// Virtual machine cannot be halted.
+	requires !halted(vm) {
+		// decode
+		var (vm',opcode) := decode(vm);
+		//
+		if opcode == ADD then stepADD(vm')
+		else if opcode == LDC then stepLDC(vm')
+		else if opcode == LOAD then stepLOAD(vm')
+		else if opcode == NOP then stepNOP(vm')
+		else if opcode == STORE then stepSTORE(vm')				
+		else 
+		 	halt(vm')
 }
 
+/**
+ * Execute an ADD instruction which pops two operands from the stack, and
+ * pushes their sum back.
+ */
+function stepADD(vm:SVM) : SVM {
+		if !halted(vm) && operands(vm,2)
+			then
+			var rhs := peek(vm,1) as int;
+			var lhs := peek(vm,2) as int;
+			var sum := (lhs + rhs) % 65536;
+			push(pop(pop(vm)),sum as u16)
+		else
+				halt(vm)
+}
+
+/**
+ * Execute an LDC instruction which pushes a constant onto the stack.
+ */
+function stepLDC(vm:SVM) : SVM {
+		if !halted(vm) && operands(vm,1) && available(vm,1)
+			then
+			// Decode operand
+			var (vm',k) := decode_operand(vm);
+			// Push operand on stack
+			push(vm',k)
+		else 
+			halt(vm)
+}
+
+/**
+ * Execute a LOAD instruction which writes the top of the stack into 
+ * a given (static) memory location.  The location is provided as an 
+ * operand.
+ */
+function stepLOAD(vm:SVM) : SVM {
+		if !halted(vm) && available(vm,1)
+			then
+			// Decode operand
+			var (vm',k) := decode_operand(vm);
+			// Sanity check valid address
+			if k < Memory.size(vm.mem)
+			// Push operand on stack
+			then push(vm',read(vm, k))
+			else
+				halt(vm')
+		else 
+				halt(vm)		
+}
+
+/**
+ * Execute a NOP instruction which leaves the SVM unchanged.
+ */
 function stepNOP(vm:SVM) : SVM { vm }
 
-function stepLDC(vm:SVM, k:u8) : SVM {
-		if size(vm.0) < capacity(vm.0)
-		then
-				svm_push(vm,k)
+/**
+ * Execute a STORE instruction which pushes the contents of a 
+ * given (static) memory location onto the stack.  The location 
+ * is provided as an operand.
+ */
+function stepSTORE(vm:SVM) : SVM {
+		if !halted(vm) && operands(vm,1)
+			then
+			// Decode operand
+			var (vm',k) := decode_operand(vm);
+			// Identify value on top of stack
+			var v := peek(vm',1);
+			// Sanity check valid address
+			if k < Memory.size(vm.mem)
+			// Write item to memory (and pop stack).
+			then write(pop(vm'), k, v)
+			else
+				halt(vm')
 		else 
-				halt(vm)
+				halt(vm)		
 }
 
 // =============================================================================
 // Microcode
 // =============================================================================
 
-function svm_decode(vm:SVM) : u8 { vm.2[vm.3] }
-
-function svm_goto(vm:SVM, k:u16) : SVM { (vm.0,vm.1,vm.2,k) }
-
-function svm_push(vm:SVM, k:u8) : SVM {
-		(push(vm.0,k as u16),vm.1,vm.2,vm.3)
+/**
+ * Check at least k operands on the stack.
+ */
+function operands(vm:SVM, k:int) : bool {
+	Stack.size(vm.stack) >= k
 }
 
-function svm_peek(vm:SVM) : u16 {
-		peek(vm.0)
+/**
+ * Check sufficient space to push k items onto the stack.
+ */
+function available(vm:SVM, k:int) : bool {
+	Stack.size(vm.stack) <= Stack.capacity(vm.stack) - k
 }
 
-function svm_pop(vm:SVM) : SVM {
-		(pop(vm.0),vm.1,vm.2,vm.3)
+/**
+ * Decode next opcode from machine.
+ */
+function decode(vm:SVM) : (SVM,u8)
+	requires !halted(vm) {
+		(goto(vm,vm.pc+1),Code.decode_u8(vm.code,vm.pc))
+}
+
+/**
+ * Decode next operand from machine.
+ */
+function decode_operand(vm:SVM) : (SVM,u16)
+	requires !halted(vm) {
+		var (vm',k) := decode(vm);
+		(vm',k as u16)
+}
+
+/**
+ * Move program counter to a given location.
+ */
+function goto(vm:SVM, k:u16) : SVM
+	requires k <= Code.size(vm.code) {
+	SVM(stack:=vm.stack,mem:=vm.mem,code:=vm.code,pc:=k)
+}
+
+/**
+ * Push byte onto stack.
+ */
+function push(vm:SVM, v:u16) : SVM
+requires Stack.size(vm.stack) < Stack.capacity(vm.stack) {
+	SVM(
+		stack:= Stack.push(vm.stack,v),
+		mem:=vm.mem,
+		code:=vm.code,
+		pc:=vm.pc)
+}
+
+/**
+ * Peek word from a given position on the stack, where "1" is the 
+ * topmost position, "2" is the next position and so on.
+ */
+function peek(vm:SVM, k:int) : u16
+  // Sanity check peek possible
+	requires k > 0 && k <= Stack.size(vm.stack) {
+		Stack.peek(vm.stack,k)
+} 
+
+/**
+ * Pop word from stack.
+ */
+function pop(vm:SVM) : SVM
+	// Cannot pop from empty stack
+	requires Stack.size(vm.stack) >= 1 {
+		SVM(stack:=Stack.pop(vm.stack),
+			mem:=vm.mem,
+			code:=vm.code,
+			pc:=vm.pc)		
+}
+
+/**
+ * Read word from data memory.
+ */
+function read(vm:SVM, k:u16) : u16
+// Address must be within bounds		
+requires k < Memory.size(vm.mem) {
+		Memory.read(vm.mem,k)
+}
+
+/**
+ * Write word into data memory.
+ */
+function write(vm:SVM, k:u16, v:u16) : SVM
+// Address must be within bounds		
+requires k < Memory.size(vm.mem) {
+		SVM(stack:=vm.stack,
+				mem:=Memory.write(vm.mem,k,v),
+				code:=vm.code,
+				pc:=vm.pc)
 }
