src/util/code.dfy
@@ -1,0 +1,34 @@
+include "int.dfy"
+
+module Code {
+	import opened Int 
+
+	// =============================================================================
+	// Code Segment
+	// =============================================================================
+
+	/**
+   * A code segment is just a sequence of words which form the 
+   * opcodes and operands of the machine instructions.
+   */
+	datatype Raw<S> = Code(contents:seq<S>)
+		
+	type T<S> = c:Raw<S> | |c.contents| < MAX_U16 witness Code([])
+
+	/**
+   * Create an empty code segment which can be used whenever we need a witness.
+   */
+	function method empty<S>() : T<S> { Code(contents:=[]) }
+
+	/**
+   * Get the size of this code segment.
+   */
+	function size<S>(c:T<S>) : u16 { |c.contents| as u16 }
+	
+	function decode_u8<S>(c:T<S>, pc:u16) : S
+		// Decode position must be valid.
+		requires pc < size(c) {
+			// Read word at given location
+			c.contents[pc]
+	}
+}
