src/util/memory.dfy
@@ -1,0 +1,45 @@
+include "int.dfy"
+
+module Memory {
+		import opened Int 
+						
+		// =============================================================================
+		// Random Access Memory
+		// =============================================================================
+		
+		datatype Raw<S> = Memory(contents:seq<S>)
+
+		type T<S> = m:Raw<S> | |m.contents| < MAX_U16
+		witness Memory([])
+
+		/**
+     * Create an empty memory which can be used whenever we need a witness.
+     */
+		function method empty<S>() : T<S> { Memory(contents:=[]) }
+
+		function size<S>(mem:T<S>) : u16 {
+				|mem.contents| as u16
+		}
+		
+		/**
+		 * Read the value at a given address in Memory.  This requires that the address 
+		 * is within bounds of the Memory.
+		 */
+		function read<S>(mem:T<S>, address:u16) : S
+			// Address must be within bounds
+			requires address < (|mem.contents| as u16) {
+				// Read location
+				mem.contents[address]
+		}
+		
+		/**
+		 * Write a value to a given address in Memory.  This requires that the address 
+		 * is within bounds of the Memory.
+		 */
+		function write<S>(mem:T<S>, address:u16, val:S) : T<S>
+			// Address must be within bounds
+			requires address < (|mem.contents| as u16) {
+				// Write location
+				Memory(contents:=mem.contents[address:=val])
+		}
+}
