src/util/stack.dfy
@@ -1,0 +1,64 @@
+include "int.dfy"
+
+module Stack {
+		import opened Int 
+
+		/**
+     * A raw stack consistents of a sequence of data, and a stack pointer.
+     */
+		datatype Raw<T> = Stack(contents:seq<T>, sp:nat)
+			
+		/**
+		 * A valid Stack: (1) must have a Stack pointer within bounds;
+		 * (2) the Stack must be addressable with 16bits.  Note, the stack 
+		 * pointer identifies the first *unused* slot on the stack.
+		 */	
+		type T<S> = s:Raw<S> | s.sp <= |s.contents| && |s.contents| <= MAX_U16
+		witness Stack([],0)
+
+		/**
+		 * Get the capacity of this Stack.
+		 */
+		function capacity<S>(st:T<S>) : int { |st.contents| }
+		
+		/**
+		 * Get the number of items currently on this Stack.
+		 */
+		function size<S>(st:T<S>) : int { st.sp }
+
+		/**
+     * Create an empty stack which can be used whenever we need a witness.
+     */
+		function method empty<S>() : T<S> { Stack(contents:=[],sp:=0) }
+		
+		/**
+		 * Push a value onto this Stack.  This requires that there is sufficient 
+		 * space for that item.
+		 */
+		function push<S>(st:T<S>, val:S) : T<S>
+				// Sanity check enough space.
+				requires size(st) < capacity(st) {
+						Stack(contents:=st.contents[st.sp:=val],sp:=st.sp+1)	
+		}
+		
+		/**
+		 * Peek nth value from top of Stack (where 1 is top item, 2 is next item, 
+     * and so on).  This requires there are sufficiently 
+     * many values.
+		 */
+		function peek<S>(st:T<S>, k:int) : S
+				// Sanity check enough items to pop!
+				requires k > 0 && k <= size(st) {
+						st.contents[st.sp-k]
+		}
+		
+		/**
+		 * Pop a value off of this Stack.  This requires that there is actually 
+		 * something to pop!
+		 */
+		function pop<S>(st:T<S>) : T<S>
+				// Sanity check something to pop.
+				requires size(st) > 0 {
+						Stack(contents:=st.contents,sp:=st.sp-1)
+		}
+}
